use Prop for env split and copy

theories/logrel_heaplang_sessions/split.v
@@ -7,39 +7,42 @@ Section EnvironmentSplitting.
   Context {Σ : gFunctors}.
   Implicit Types A : lty Σ.
 
-  (* TODO: Should this be an iProp or just a Prop? Is it ever the case that splitting an environment is only allowed when you have some resource? *)
-  Definition env_split Γ Γ1 Γ2 : iProp Σ := (□ ∀ vs, env_ltyped Γ vs -∗ env_ltyped Γ1 vs ∗ env_ltyped Γ2 vs)%I.
+  Definition env_split Γ Γ1 Γ2 : Prop :=
+    ((∀ vs, env_ltyped Γ vs -∗ env_ltyped Γ1 vs ∗ env_ltyped Γ2 vs)%I : iProp Σ).
 
   Lemma env_split_empty:
     env_split ∅ ∅ ∅.
   Proof.
-    iIntros (vs) "!> H".
+    iStartProof. iIntros (vs) "HΓ".
     iSplitL; by rewrite /env_ltyped big_sepM_empty.
   Qed.
 
   Lemma env_split_left Γ Γ1 Γ2 x A:
-    Γ !! x = None → env_split Γ Γ1 Γ2 -∗ env_split (<[x := A]> Γ) (<[x := A]> Γ1) Γ2.
+    Γ !! x = None →
+    env_split Γ Γ1 Γ2 →
+    env_split (<[x := A]> Γ) (<[x := A]> Γ1) Γ2.
   Proof.
-    intros HΓx.
-    iIntros "#Hsplit" (vs) "!> HΓ".
+    intros HΓx Hsplit.
+    iStartProof. iIntros (vs) "HΓ".
     iPoseProof (big_sepM_insert with "HΓ") as "[Hv HΓ]"; try assumption.
-    iPoseProof ("Hsplit" with "HΓ") as "[HΓ1 HΓ2]". iFrame.
+    iPoseProof (Hsplit with "HΓ") as "[HΓ1 HΓ2]". iFrame.
     iApply (big_sepM_insert_2 with "[Hv]"); simpl; iFrame.
   Qed.
 
   Lemma env_split_comm Γ Γ1 Γ2:
-    env_split Γ Γ1 Γ2 -∗ env_split Γ Γ2 Γ1.
+    env_split Γ Γ1 Γ2 → env_split Γ Γ2 Γ1.
   Proof.
-    iIntros "#Hsplit" (vs) "!> HΓ".
-    iDestruct ("Hsplit" with "HΓ") as "[HΓ1 HΓ2]".
+    intros Hsplit. iStartProof. iIntros (vs) "HΓ".
+    iDestruct (Hsplit with "HΓ") as "[HΓ1 HΓ2]".
     iFrame.
   Qed.
 
   Lemma env_split_right Γ Γ1 Γ2 x A:
-    Γ !! x = None → env_split Γ Γ1 Γ2 -∗ env_split (<[x := A]> Γ) Γ1 (<[x := A]> Γ2).
+    Γ !! x = None →
+    env_split Γ Γ1 Γ2 →
+    env_split (<[x := A]> Γ) Γ1 (<[x := A]> Γ2).
   Proof.
-    intros HΓx.
-    iIntros "#Hsplit".
+    intros HΓx Hsplit. iStartProof.
     iApply env_split_comm.
     iApply env_split_left; try assumption.
       by iApply env_split_comm.
@@ -47,15 +50,19 @@ Section EnvironmentSplitting.
 
   (* TODO: Get rid of side condition that x does not appear in Γ *)
   Lemma env_split_copy Γ Γ1 Γ2 (x : string) A:
-    Γ !! x = None → LTyCopy A → env_split Γ Γ1 Γ2 -∗ env_split (<[x := A]> Γ) (<[x := A]> Γ1) (<[x := A]> Γ2).
+    Γ !! x = None →
+    LTyCopy A →
+    env_split Γ Γ1 Γ2 →
+    env_split (<[x := A]> Γ) (<[x := A]> Γ1) (<[x := A]> Γ2).
   Proof.
-    intros Hcopy HΓx. iIntros "#Hsplit" (vs) "!> HΓ".
+    intros Hcopy HΓx Hsplit. iIntros (vs) "HΓ".
     iPoseProof (big_sepM_insert with "HΓ") as "[Hv HΓ]"; try assumption.
     iDestruct "Hv" as (v ?) "#HAv".
-    iPoseProof ("Hsplit" with "HΓ") as "[HΓ1 HΓ2]".
+    iPoseProof (Hsplit with "HΓ") as "[HΓ1 HΓ2]".
     iSplitL "HΓ1"; iApply big_sepM_insert_2; simpl; iFrame; eauto.
   Qed.
 
-  (* TODO: Should this be a Prop, just like env_split perhaps? *)
-  Definition env_copy Γ Γ' : iProp Σ := (□ (∀ vs, env_ltyped Γ vs -∗ □ env_ltyped Γ' vs))%I.
+  (* TODO: Prove lemmas about this *)
+  Definition env_copy Γ Γ' : Prop :=
+    ((∀ vs, env_ltyped Γ vs -∗ □ env_ltyped Γ' vs) : iProp Σ)%I.
 End EnvironmentSplitting.
